feat(imp): finish

lf/Imp.v
@@ -464,13 +464,26 @@ Admitted.
     it is sound.  Use the tacticals we've just seen to make the proof
     as short and elegant as possible. *)
 
-Fixpoint optimize_0plus_b (b : bexp) : bexp
-  (* REPLACE THIS LINE WITH ":= _your_definition_ ." *). Admitted.
+Fixpoint optimize_0plus_b (b : bexp) : bexp :=
+  match b with
+  | BTrue | BFalse => b
+  | BEq e1 e2 => BEq (optimize_0plus e1) (optimize_0plus e2)
+  | BNeq e1 e2 => BNeq (optimize_0plus e1) (optimize_0plus e2)
+  | BLe e1 e2 => BLe (optimize_0plus e1) (optimize_0plus e2)
+  | BGt e1 e2 => BGt (optimize_0plus e1) (optimize_0plus e2)
+  | BNot e => BNot (optimize_0plus_b e)
+  | BAnd e1 e2 => BAnd (optimize_0plus_b e1) (optimize_0plus_b e2)
+  end.
 
 Theorem optimize_0plus_b_sound : forall b,
   beval (optimize_0plus_b b) = beval b.
 Proof.
-  (* FILL IN HERE *) Admitted.
+  intros b.
+  induction b;
+    try (simpl; repeat rewrite optimize_0plus_sound; reflexivity).
+  - simpl. rewrite IHb. reflexivity.
+  - simpl. rewrite IHb1. rewrite IHb2. reflexivity.
+Qed.
 (** [] *)
 
 (** **** Exercise: 4 stars, standard, optional (optimize)
@@ -483,9 +496,27 @@ Proof.
     optimization and its correctness proof -- and build up
     incrementally to something more interesting.)  *)
 
-(* FILL IN HERE
+Fixpoint optimize_short_circuit_left (b : bexp) : bexp :=
+  match b with
+  | BTrue | BFalse | BEq _ _ | BNeq _ _ | BLe _ _ | BGt _ _ => b
+  | BNot e => BNot (optimize_short_circuit_left e)
+  | BAnd BFalse _ => BFalse
+  | BAnd e1 e2 =>
+    BAnd (optimize_short_circuit_left e1) (optimize_short_circuit_left e2)
+  end.
 
-    [] *)
+Theorem optimize_short_circuit_sound : forall b,
+  beval (optimize_short_circuit_left b) = beval b.
+Proof.
+  intros b.
+  induction b;
+    try reflexivity.
+  - simpl. rewrite IHb. reflexivity.
+  - destruct b1; try (simpl; simpl in IHb1; try rewrite IHb1; try rewrite IHb2;
+                      reflexivity).
+Qed.
+(** [] *)
+
 
 (* ================================================================= *)
 (** ** Defining New Tactics *)
@@ -778,7 +809,42 @@ Inductive aevalR : aexp -> nat -> Prop :=
 
     Write out a corresponding definition of boolean evaluation as a
     relation (in inference rule notation). *)
-(* FILL IN HERE *)
+(*
+                             -------------                            (E_BTrue)
+                             BTrue ==> true
+
+                            ---------------                          (E_BFalse)
+                            BFalse ==> false
+
+                               e1 ==> n1
+                               e2 ==> n2
+                         -------------------                            (E_BEq)
+                         BEq e1 e2 ==> n1=?n2
+
+                               e1 ==> n1
+                               e2 ==> n2
+                      ---------------------------                      (E_BNeq)
+                      BNeq e1 e2 ==> negb (n1=?n2)
+
+                               e1 ==> n1
+                               e2 ==> n2
+                         --------------------                           (E_BLe)
+                         BLe e1 e2 ==> n1<=?n2
+
+                               e1 ==> n1
+                               e2 ==> n2
+                      ---------------------------                       (E_BGt)
+                      BGt e1 e2 ==> negb (n1<=?n2)
+
+                                e ==> b
+                           ----------------                            (E_BNot)
+                           BNot e ==> negb b
+
+                               e1 ==> b1
+                               e2 ==> b2
+                         --------------------                          (E_BAnd)
+                         BAnd b1 b2 ==> b1&&b2
+*)
 
 (* Do not modify the following line: *)
 Definition manual_grade_for_beval_rules : option (nat*string) := None.
@@ -848,14 +914,44 @@ Qed.
 
 Reserved Notation "e '==>b' b" (at level 90, left associativity).
 Inductive bevalR: bexp -> bool -> Prop :=
-(* FILL IN HERE *)
-where "e '==>b' b" := (bevalR e b) : type_scope
-.
+  | E_BTrue : BTrue ==>b true
+  | E_BFalse : BFalse ==>b false
+  | E_BEq (e1 e2 : aexp) (n1 n2 : nat) :
+      (e1 ==> n1) ->
+      (e2 ==> n2) ->
+      (BEq e1 e2) ==>b (n1 =? n2)
+  | E_BNeq (e1 e2 : aexp) (n1 n2 : nat) :
+      (e1 ==> n1) ->
+      (e2 ==> n2) ->
+      (BNeq e1 e2) ==>b (negb (n1 =? n2))
+  | E_BLe (e1 e2 : aexp) (n1 n2 : nat) :
+      (e1 ==> n1) ->
+      (e2 ==> n2) ->
+      (BLe e1 e2) ==>b (n1 <=? n2)
+  | E_BGt (e1 e2 : aexp) (n1 n2 : nat) :
+      (e1 ==> n1) ->
+      (e2 ==> n2) ->
+      (BGt e1 e2) ==>b (negb (n1 <=? n2))
+  | E_BNot (e : bexp) (b : bool) :
+      (e ==>b b) -> (BNot e) ==>b (negb b)
+  | E_BAnd (e1 e2 : bexp) (b1 b2 : bool) :
+      (e1 ==>b b1) ->
+      (e2 ==>b b2) ->
+      (BAnd e1 e2) ==>b (b1 && b2)
+
+  where "e '==>b' b" := (bevalR e b) : type_scope.
 
 Lemma beval_iff_bevalR : forall b bv,
   b ==>b bv <-> beval b = bv.
 Proof.
-  (* FILL IN HERE *) Admitted.
+  split.
+  - intros H. induction H;
+    simpl; try rewrite aeval_iff_aevalR in *; subst; reflexivity.
+  - generalize dependent bv.
+    induction b; simpl; intros; subst; constructor;
+      try rewrite aeval_iff_aevalR; try apply IHb; try apply IHb1;
+      try apply IHb2; reflexivity.
+Qed.
 (** [] *)
 
 End AExp.
@@ -1542,7 +1638,11 @@ Example ceval_example2:
     Z := 2
   ]=> (Z !-> 2 ; Y !-> 1 ; X !-> 0).
 Proof.
-  (* FILL IN HERE *) Admitted.
+  apply E_Seq with (X !-> 0).
+  - apply E_Asgn. reflexivity.
+  - apply E_Seq with (Y !-> 1 ; X !-> 0);
+    apply E_Asgn; reflexivity.
+Qed.
 (** [] *)
 
 Set Printing Implicit.
@@ -1556,15 +1656,30 @@ Check @ceval_example2.
     which you can reverse-engineer to discover the program you should
     write.  The proof of that theorem will be somewhat lengthy. *)
 
-Definition pup_to_n : com
-  (* REPLACE THIS LINE WITH ":= _your_definition_ ." *). Admitted.
+Definition pup_to_n : com := <{
+  Y := 0;
+  while (X > 0) do
+    Y := Y + X;
+    X := X - 1
+  end
+}>.
 
 Theorem pup_to_2_ceval :
   (X !-> 2) =[
     pup_to_n
   ]=> (X !-> 0 ; Y !-> 3 ; X !-> 1 ; Y !-> 2 ; Y !-> 0 ; X !-> 2).
 Proof.
-  (* FILL IN HERE *) Admitted.
+  apply E_Seq with (Y !-> 0 ; X !-> 2); try (apply E_Asgn; reflexivity).
+  apply E_WhileTrue with (X !-> 1 ; Y !-> 2 ; Y !-> 0 ; X !-> 2);
+    try (apply E_Seq with (Y !-> 2 ; Y !-> 0 ; X !-> 2); apply E_Asgn);
+    try reflexivity.
+  apply E_WhileTrue with (X !-> 0 ; Y !-> 3; X !-> 1 ; Y !-> 2 ; Y !-> 0 ;
+                          X !-> 2);
+    try (apply E_Seq with (Y !-> 3; X !-> 1 ; Y !-> 2 ; Y !-> 0 ; X !-> 2);
+        apply E_Asgn);
+    try reflexivity.
+  apply E_WhileFalse. reflexivity.
+Qed.
 (** [] *)
 
 (* ================================================================= *)
@@ -1640,7 +1755,16 @@ Proof.
 
     State and prove a specification of [XtimesYinZ]. *)
 
-(* FILL IN HERE *)
+Theorem XtimesYinZ_spec : forall st n1 n2 st',
+  st X = n1 ->
+  st Y = n2 ->
+  st =[ XtimesYinZ ]=> st' ->
+  st' Z = n1 * n2.
+Proof.
+  intros st n1 n2 st' HX HY Heval.
+  inversion Heval. subst. clear Heval. simpl.
+  apply t_update_eq.
+Qed.
 
 (* Do not modify the following line: *)
 Definition manual_grade_for_XtimesYinZ_spec : option (nat*string) := None.
@@ -1659,7 +1783,10 @@ Proof.
       contradictory and so can be solved in one step with
       [discriminate]. *)
 
-  (* FILL IN HERE *) Admitted.
+  induction contra; try discriminate.
+  - inversion Heqloopdef. subst. discriminate.
+  - apply IHcontra2. apply Heqloopdef.
+Qed.
 (** [] *)
 
 (** **** Exercise: 3 stars, standard (no_whiles_eqv)
@@ -1686,13 +1813,32 @@ Fixpoint no_whiles (c : com) : bool :=
     while loops.  Then prove its equivalence with [no_whiles]. *)
 
 Inductive no_whilesR: com -> Prop :=
- (* FILL IN HERE *)
-.
+  | NW_Skip :
+      no_whilesR <{ skip }>
+  | NW_Asgn : forall a x,
+      no_whilesR <{ x := a }>
+  | NW_If : forall b ct cf,
+      no_whilesR ct ->
+      no_whilesR cf ->
+      no_whilesR <{ if b then ct else cf end }>
+  | NW_Seq : forall c1 c2,
+      no_whilesR c1 ->
+      no_whilesR c2 ->
+      no_whilesR <{ c1 ; c2 }>.
 
 Theorem no_whiles_eqv:
   forall c, no_whiles c = true <-> no_whilesR c.
 Proof.
-  (* FILL IN HERE *) Admitted.
+  split.
+  - induction c; intros H; inversion H; constructor;
+      try apply IHc1; remember (no_whiles c1) as b1;
+      try apply IHc2; remember (no_whiles c2) as b2;
+      try (destruct b1; try reflexivity; discriminate);
+      try (destruct b2; try reflexivity; rewrite andb_comm in *; discriminate).
+  - intros H. induction H;
+      try (simpl; rewrite IHno_whilesR1; rewrite IHno_whilesR2);
+      reflexivity.
+Qed.
 (** [] *)
 
 (** **** Exercise: 4 stars, standard (no_whiles_terminating)
@@ -1702,7 +1848,22 @@ Proof.
 
     Use either [no_whiles] or [no_whilesR], as you prefer. *)
 
-(* FILL IN HERE *)
+Theorem no_whiles_terminating:
+  forall c st, no_whilesR c -> exists st', st =[ c ]=> st'.
+Proof.
+  intros. generalize dependent st.
+  induction H.
+  - intros st. exists st. constructor.
+  - intros st. exists (x !-> (aeval st a) ; st). constructor. reflexivity.
+  - intros st. destruct (beval st b) eqn:EQ.
+    + destruct (IHno_whilesR1 st) as [st' IH]. exists st'.
+      apply E_IfTrue; [apply EQ | apply IH].
+    + destruct (IHno_whilesR2 st) as [st' IH]. exists st'.
+      apply E_IfFalse; [apply EQ | apply IH].
+  - intros st. destruct (IHno_whilesR1 st) as [st' IH1].
+    destruct (IHno_whilesR2 st') as [st'' IH2]. exists st''.
+    apply E_Seq with st'; [apply IH1 | apply IH2].
+Qed.
 
 (* Do not modify the following line: *)
 Definition manual_grade_for_no_whiles_terminating : option (nat*string) := None.
@@ -1771,10 +1932,39 @@ Inductive sinstr : Type :=
     But for sake of later exercises, it would be best to skip the
     offending instruction and continue with the next one.  *)
 
+Definition s_poptwo (stack : list nat) : option (nat*nat*(list nat)) :=
+  match stack with
+  | n1 :: stack' =>
+      match stack' with
+      | n2 :: stack'' => Some (n1, n2, stack'')
+      | [] => None
+      end
+  | [] => None
+  end.
+
 Fixpoint s_execute (st : state) (stack : list nat)
                    (prog : list sinstr)
-                 : list nat
-  (* REPLACE THIS LINE WITH ":= _your_definition_ ." *). Admitted.
+                 : list nat :=
+  match prog with
+  | [] => stack
+  | (SPush n) :: prog' => s_execute st (n :: stack) prog'
+  | (SLoad x) :: prog' => s_execute st ((st x) :: stack) prog'
+  | SPlus :: prog' =>
+      match s_poptwo stack with
+      | Some (n1, n2, stack') => s_execute st ((n2 + n1) :: stack') prog'
+      | None => s_execute st stack prog'
+      end
+  | SMinus :: prog' =>
+      match s_poptwo stack with
+      | Some (n1, n2, stack') => s_execute st ((n2 - n1) :: stack') prog'
+      | None => s_execute st stack prog'
+      end
+  | SMult :: prog' =>
+      match s_poptwo stack with
+      | Some (n1, n2, stack') => s_execute st ((n2 * n1) :: stack') prog'
+      | None => s_execute st stack prog'
+      end
+  end.
 
 Check s_execute.
 
@@ -1782,20 +1972,30 @@ Example s_execute1 :
      s_execute empty_st []
        [SPush 5; SPush 3; SPush 1; SMinus]
    = [2; 5].
-(* FILL IN HERE *) Admitted.
+Proof.
+  reflexivity.
+Qed.
 
 Example s_execute2 :
      s_execute (X !-> 3) [3;4]
        [SPush 4; SLoad X; SMult; SPlus]
    = [15; 4].
-(* FILL IN HERE *) Admitted.
+Proof.
+  reflexivity.
+Qed.
 
 (** Next, write a function that compiles an [aexp] into a stack
     machine program. The effect of running the program should be the
     same as pushing the value of the expression on the stack. *)
 
-Fixpoint s_compile (e : aexp) : list sinstr
-  (* REPLACE THIS LINE WITH ":= _your_definition_ ." *). Admitted.
+Fixpoint s_compile (e : aexp) : list sinstr :=
+  match e with
+  | ANum n => [SPush n]
+  | AId x => [SLoad x]
+  | <{a1 + a2}> => (s_compile a1) ++ (s_compile a2) ++ [SPlus]
+  | <{a1 - a2}> => (s_compile a1) ++ (s_compile a2) ++ [SMinus]
+  | <{a1 * a2}> => (s_compile a1) ++ (s_compile a2) ++ [SMult]
+  end.
 
 (** After you've defined [s_compile], prove the following to test
     that it works. *)
@@ -1803,7 +2003,9 @@ Fixpoint s_compile (e : aexp) : list sinstr
 Example s_compile1 :
   s_compile <{ X - (2 * Y) }>
   = [SLoad X; SPush 2; SLoad Y; SMult; SMinus].
-(* FILL IN HERE *) Admitted.
+Proof.
+  reflexivity.
+Qed.
 (** [] *)
 
 (** **** Exercise: 3 stars, standard (execute_app) *)
@@ -1816,8 +2018,12 @@ Example s_compile1 :
 Theorem execute_app : forall st p1 p2 stack,
   s_execute st stack (p1 ++ p2) = s_execute st (s_execute st stack p1) p2.
 Proof.
-  (* FILL IN HERE *) Admitted.
-
+  intros st p1. generalize dependent st. induction p1 as [| i p1' IH].
+  - intros. reflexivity.
+  - intros. destruct i; simpl; try apply IH;
+      try (destruct stack as [| n1 stack']; simpl; try apply IH;
+           destruct stack' as [| n2 stack'']; simpl; try apply IH).
+Qed.
 (** [] *)
 
 (** **** Exercise: 3 stars, standard (stack_compiler_correct) *)
@@ -1830,14 +2036,19 @@ Proof.
 Lemma s_compile_correct_aux : forall st e stack,
   s_execute st stack (s_compile e) = aeval st e :: stack.
 Proof.
-  (* FILL IN HERE *) Admitted.
+  intros st e. generalize dependent st.
+  induction e; intros;
+    try (simpl; repeat rewrite execute_app; rewrite IHe1; rewrite IHe2);
+    try reflexivity.
+Qed.
 
 (** The main theorem should be a very easy corollary of that lemma. *)
 
 Theorem s_compile_correct : forall (st : state) (e : aexp),
   s_execute st [] (s_compile e) = [ aeval st e ].
 Proof.
-  (* FILL IN HERE *) Admitted.
+  intros. apply s_compile_correct_aux.
+Qed.
 
 (** [] *)
 
@@ -1858,9 +2069,24 @@ Proof.
     would _not_ be equivalent to the original, since it would make more
     programs terminate.) *)
 
-(* FILL IN HERE
+Fixpoint beval_shortcircuit (st : state) (b : bexp) : bool :=
+  match b with
+  | <{~ b1}> => negb (beval_shortcircuit st b1)
+  | <{b1 && b2}> =>
+      if beval_shortcircuit st b1
+      then beval_shortcircuit st b2
+      else false
+  | _ => beval st b
+  end.
 
-    [] *)
+Theorem beval_shortciruit_equiv:
+  forall st b, beval_shortcircuit st b = beval st b.
+Proof.
+  intros. induction b; try reflexivity.
+  - simpl. rewrite IHb. reflexivity.
+  - simpl. rewrite IHb1. rewrite IHb2. unfold andb. reflexivity.
+Qed.
+(** [] *)
 
 Module BreakImp.
 (** **** Exercise: 4 stars, advanced (break_imp)
@@ -1982,7 +2208,38 @@ Reserved Notation "st '=[' c ']=>' st' '/' s"
 Inductive ceval : com -> state -> result -> state -> Prop :=
   | E_Skip : forall st,
       st =[ CSkip ]=> st / SContinue
-  (* FILL IN HERE *)
+  | E_Break : forall st,
+      st =[ CBreak ]=> st / SBreak
+  | E_Asgn : forall st a n x,
+      aeval st a = n ->
+      st =[ x := a ]=> (x !-> n ; st) / SContinue
+  | E_SeqBreak : forall c1 c2 st st',
+      st =[ c1 ]=> st' / SBreak ->
+      st =[ c1 ; c2 ]=> st' / SBreak
+  | E_SeqContinue : forall c1 c2 st st' st'' s,
+      st =[ c1 ]=> st' / SContinue ->
+      st' =[ c2 ]=> st'' / s ->
+      st =[ c1 ; c2 ]=> st'' / s
+  | E_IfTrue : forall st st' s b c1 c2,
+      beval st b = true ->
+      st =[ c1 ]=> st' / s ->
+      st =[ if b then c1 else c2 end ]=> st' / s
+  | E_IfFalse : forall st st' s b c1 c2,
+      beval st b = false ->
+      st =[ c2 ]=> st' / s ->
+      st =[ if b then c1 else c2 end]=> st' / s
+  | E_WhileFalse : forall b st c,
+      beval st b = false ->
+      st =[ while b do c end ]=> st / SContinue
+  | E_WhileTrueBreak : forall st st' b c,
+      beval st b = true ->
+      st =[ c ]=> st' / SBreak ->
+      st =[ while b do c end ]=> st' / SContinue
+  | E_WhileTrueContinue : forall st st' st'' b c,
+      beval st b = true ->
+      st =[ c ]=> st' / SContinue ->
+      st' =[ while b do c end ]=> st'' / SContinue ->
+      st =[ while b do c end ]=> st'' / SContinue
 
   where "st '=[' c ']=>' st' '/' s" := (ceval c st s st').
 
@@ -1992,33 +2249,40 @@ Theorem break_ignore : forall c st st' s,
      st =[ break; c ]=> st' / s ->
      st = st'.
 Proof.
-  (* FILL IN HERE *) Admitted.
+  intros. inversion H; subst.
+  - inversion H5. reflexivity.
+  - inversion H2.
+Qed.
 
 Theorem while_continue : forall b c st st' s,
   st =[ while b do c end ]=> st' / s ->
   s = SContinue.
 Proof.
-  (* FILL IN HERE *) Admitted.
+  intros. inversion H; subst; try reflexivity.
+Qed.
 
 Theorem while_stops_on_break : forall b c st st',
   beval st b = true ->
   st =[ c ]=> st' / SBreak ->
   st =[ while b do c end ]=> st' / SContinue.
 Proof.
-  (* FILL IN HERE *) Admitted.
+  intros. apply E_WhileTrueBreak; assumption.
+Qed.
 
 Theorem seq_continue : forall c1 c2 st st' st'',
   st =[ c1 ]=> st' / SContinue ->
   st' =[ c2 ]=> st'' / SContinue ->
   st =[ c1 ; c2 ]=> st'' / SContinue.
 Proof.
-  (* FILL IN HERE *) Admitted.
+  intros. apply E_SeqContinue with st'; assumption.
+Qed.
 
 Theorem seq_stops_on_break : forall c1 c2 st st',
   st =[ c1 ]=> st' / SBreak ->
   st =[ c1 ; c2 ]=> st' / SBreak.
 Proof.
-  (* FILL IN HERE *) Admitted.
+  intros. apply E_SeqBreak. assumption.
+Qed.
 (** [] *)
 
 (** **** Exercise: 3 stars, advanced, optional (while_break_true) *)
@@ -2027,7 +2291,12 @@ Theorem while_break_true : forall b c st st',
   beval st' b = true ->
   exists st'', st'' =[ c ]=> st' / SBreak.
 Proof.
-(* FILL IN HERE *) Admitted.
+  intros. remember (<{ while b do c end }>) as loop.
+  induction H; try discriminate; inversion Heqloop; subst.
+  - rewrite H in *. discriminate.
+  - exists st. apply H1.
+  - apply IHceval2; try reflexivity; try assumption.
+Qed.
 (** [] *)
 
 (** **** Exercise: 4 stars, advanced, optional (ceval_deterministic) *)
@@ -2036,7 +2305,33 @@ Theorem ceval_deterministic: forall (c:com) st st1 st2 s1 s2,
      st =[ c ]=> st2 / s2 ->
      st1 = st2 /\ s1 = s2.
 Proof.
-  (* FILL IN HERE *) Admitted.
+  intros c st st1 st2 s1 s2 E1 E2.
+  generalize dependent s2. generalize dependent st2.
+  induction E1; intros st2 s2 E2.
+  - inversion E2. split; reflexivity.
+  - inversion E2. split; reflexivity.
+  - inversion E2. subst. split; reflexivity.
+  - apply IHE1. inversion E2; subst; try apply H4. apply IHE1 in H1.
+    destruct H1 as [_ Hcontra]. discriminate.
+  - apply IHE1_2. inversion E2; subst.
+    + apply IHE1_1 in H4. destruct H4 as [_ Hcontra]. discriminate.
+    + apply IHE1_1 in H1. destruct H1 as [H1 _]. subst. assumption.
+  - apply IHE1.
+    inversion E2; subst; try apply H7; rewrite H in *; discriminate.
+  - apply IHE1.
+    inversion E2; subst; rewrite H in *; try discriminate; apply H7.
+  - inversion E2; subst; try (split; reflexivity);
+      rewrite H in *; discriminate.
+  - inversion E2; subst.
+    + rewrite H in *. discriminate.
+    + apply IHE1 in H6. destruct H6 as [H6 _].
+      split; try reflexivity; try assumption.
+    + apply IHE1 in H3. destruct H3 as [_ Hcontra]. discriminate.
+  - apply IHE1_2. inversion E2; subst.
+    + rewrite H in *. discriminate.
+    + apply IHE1_1 in H6. destruct H6 as [_ Hcontra]. discriminate.
+    + apply IHE1_1 in H3. destruct H3 as [H3 _]. subst. assumption.
+Qed.
 
 (** [] *)
 End BreakImp.
@@ -2055,9 +2350,124 @@ End BreakImp.
     that makes up the body of the loop.  (You don't need to worry
     about making up a concrete Notation for [for] loops, but feel free
     to play with this too if you like.) *)
+Module ForImp.
 
-(* FILL IN HERE
+Inductive com : Type :=
+  | CSkip
+  | CBreak
+  | CAsgn (x : string) (a : aexp)
+  | CSeq (c1 c2 : com)
+  | CIf (b : bexp) (c1 c2 : com)
+  | CWhile (b : bexp) (c : com)
+  | CFor (cinit : com) (ccond : bexp) (cend : com) (c : com).
 
-    [] *)
+Notation "'break'" := CBreak (in custom com at level 0).
+Notation "'skip'"  :=
+         CSkip (in custom com at level 0) : com_scope.
+Notation "x := y"  :=
+         (CAsgn x y)
+            (in custom com at level 0, x constr at level 0,
+             y at level 85, no associativity) : com_scope.
+Notation "x ; y" :=
+         (CSeq x y)
+           (in custom com at level 90, right associativity) : com_scope.
+Notation "'if' x 'then' y 'else' z 'end'" :=
+         (CIf x y z)
+           (in custom com at level 89, x at level 99,
+            y at level 99, z at level 99) : com_scope.
+Notation "'while' x 'do' y 'end'" :=
+         (CWhile x y)
+            (in custom com at level 89, x at level 99, y at level 99) : com_scope.
+Notation "'for' w 'until' x 'after' y 'do' z 'end'" :=
+         (CFor w x y z)
+            (in custom com at level 89, w at level 99,
+             x at level 99, y at level 99, z at level 99) : com_scope.
+
+Inductive result : Type :=
+  | SContinue
+  | SBreak.
+
+Reserved Notation "st '=[' c ']=>' st' '/' s"
+     (at level 40, c custom com at level 99, st' constr at next level).
+
+Inductive ceval : com -> state -> result -> state -> Prop :=
+  | E_Skip : forall st,
+      st =[ CSkip ]=> st / SContinue
+  | E_Break : forall st,
+      st =[ CBreak ]=> st / SBreak
+  | E_Asgn : forall st a n x,
+      aeval st a = n ->
+      st =[ x := a ]=> (x !-> n ; st) / SContinue
+  | E_SeqBreak : forall c1 c2 st st',
+      st =[ c1 ]=> st' / SBreak ->
+      st =[ c1 ; c2 ]=> st' / SBreak
+  | E_SeqContinue : forall c1 c2 st st' st'' s,
+      st =[ c1 ]=> st' / SContinue ->
+      st' =[ c2 ]=> st'' / s ->
+      st =[ c1 ; c2 ]=> st'' / s
+  | E_IfTrue : forall st st' s b c1 c2,
+      beval st b = true ->
+      st =[ c1 ]=> st' / s ->
+      st =[ if b then c1 else c2 end ]=> st' / s
+  | E_IfFalse : forall st st' s b c1 c2,
+      beval st b = false ->
+      st =[ c2 ]=> st' / s ->
+      st =[ if b then c1 else c2 end]=> st' / s
+  | E_WhileFalse : forall b st c,
+      beval st b = false ->
+      st =[ while b do c end ]=> st / SContinue
+  | E_WhileTrueBreak : forall st st' b c,
+      beval st b = true ->
+      st =[ c ]=> st' / SBreak ->
+      st =[ while b do c end ]=> st' / SContinue
+  | E_WhileTrueContinue : forall st st' st'' b c,
+      beval st b = true ->
+      st =[ c ]=> st' / SContinue ->
+      st' =[ while b do c end ]=> st'' / SContinue ->
+      st =[ while b do c end ]=> st'' / SContinue
+  | E_For : forall st st' st'' cinit b c cend,
+      st =[ cinit ]=> st' / SContinue ->
+      st' =[ while b do c ; cend end ]=> st'' / SContinue ->
+      st =[ for cinit until b after cend do c end ]=> st'' / SContinue
+
+  where "st '=[' c ']=>' st' '/' s" := (ceval c st s st').
+
+Theorem ceval_deterministic: forall (c:com) st st1 st2 s1 s2,
+     st =[ c ]=> st1 / s1 ->
+     st =[ c ]=> st2 / s2 ->
+     st1 = st2 /\ s1 = s2.
+Proof.
+  intros c st st1 st2 s1 s2 E1 E2.
+  generalize dependent s2. generalize dependent st2.
+  induction E1; intros st2 s2 E2.
+  - inversion E2. split; reflexivity.
+  - inversion E2. split; reflexivity.
+  - inversion E2. subst. split; reflexivity.
+  - apply IHE1. inversion E2; subst; try apply H4. apply IHE1 in H1.
+    destruct H1 as [_ Hcontra]. discriminate.
+  - apply IHE1_2. inversion E2; subst.
+    + apply IHE1_1 in H4. destruct H4 as [_ Hcontra]. discriminate.
+    + apply IHE1_1 in H1. destruct H1 as [H1 _]. subst. assumption.
+  - apply IHE1.
+    inversion E2; subst; try apply H7; rewrite H in *; discriminate.
+  - apply IHE1.
+    inversion E2; subst; rewrite H in *; try discriminate; apply H7.
+  - inversion E2; subst; try (split; reflexivity);
+      rewrite H in *; discriminate.
+  - inversion E2; subst.
+    + rewrite H in *. discriminate.
+    + apply IHE1 in H6. destruct H6 as [H6 _].
+      split; try reflexivity; try assumption.
+    + apply IHE1 in H3. destruct H3 as [_ Hcontra]. discriminate.
+  - apply IHE1_2. inversion E2; subst.
+    + rewrite H in *. discriminate.
+    + apply IHE1_1 in H6. destruct H6 as [_ Hcontra]. discriminate.
+    + apply IHE1_1 in H3. destruct H3 as [H3 _]. subst. assumption.
+  - apply IHE1_2. inversion E2. subst. apply IHE1_1 in H6.
+    destruct H6 as [H6 _]. subst. assumption.
+Qed.
+
+End ForImp.
+(** [] *)
 
 (* 2023-03-25 11:11 *)
